src/tls/HKDF.fst
@@ -3,12 +3,12 @@ TLS 1.3 HKDF extract and expand constructions, parametrized by their hash algori
 *)
 module HKDF
 
+open Mem
 open FStar.UInt32
+open Hashing.Spec
 open FStar.Bytes
 
-open Hashing.Spec
-open TLSConstants
-open Parse
+//open Parse
 
 private let max (a:int) (b:int) = if a < b then b else a
 
@@ -30,15 +30,17 @@ HKDF-Extract(salt, IKM) -> PRK
    PRK = HMAC-Hash(salt, IKM)
 *)
 
+inline_for_extraction
 val extract: 
-  #ha: Hashing.alg -> salt: hkey ha -> 
+  #ha: EverCrypt.HMAC.ha -> 
+  salt: hkey ha -> 
   ikm: macable ha -> 
   ST (hkey ha)
   (requires (fun h0 -> True))
   (ensures (fun h0 t h1 -> FStar.HyperStack.modifies Set.empty h0 h1))
 
+inline_for_extraction
 let extract #ha salt ikm = HMAC.hmac ha salt ikm
-
 
 (*-------------------------------------------------------------------*)
 (*
@@ -67,6 +69,52 @@ HKDF-Expand(PRK, info, L) -> OKM
    ...
 *)
 
+
+val expand: 
+  #ha:Hashing.alg -> 
+  prk: hkey ha ->
+  info: bytes -> 
+  len: UInt32.t {v len <= op_Multiply 255 (tagLength ha)} ->
+  Stack (lbytes32 len)
+  (requires (fun h0 -> True))
+  (ensures (fun h0 t h1 -> modifies Set.empty h0 h1))
+
+#reset-options "--admit_smt_queries true"
+let expand #ha prk info len =
+  let h00 = HyperStack.ST.get() in 
+  push_frame(); 
+  let tlen = EverCrypt.Hash.tagLen ha in
+  let prk_p = LowStar.Buffer.alloca 0uy tlen in 
+  store_bytes prk prk_p;
+  assert_norm(EverCrypt.HMAC.keysized ha (EverCrypt.Hash.tagLength ha));
+
+  let tag_p = LowStar.Buffer.alloca 0uy tlen in
+
+  let infolen = Bytes.len info in 
+
+  if infolen = 0ul then (
+    let info_p = LowStar.Buffer.null in 
+    EverCrypt.HKDF.hkdf_expand ha tag_p prk_p tlen info_p infolen tlen
+  )
+  else (
+    push_frame();
+    let info_p = LowStar.Buffer.alloca 0uy infolen in 
+    store_bytes info info_p;
+    EverCrypt.HKDF.hkdf_expand ha tag_p prk_p tlen info_p infolen tlen;
+    pop_frame()
+    );
+  assume False;//18-09-01 not sure what's broken
+    
+  let tag = of_buffer tlen prk_p in
+  pop_frame();
+  let h11 = HyperStack.ST.get() in 
+  //18-09-01 todo, as in Hashing.compute
+  //assume(HyperStack.modifies Set.empty h00 h11);
+  tag
+
+
+(* earlier, bytes-level implementation:
+
 /// Generates enough bytes by concatenating HMAC blocks;
 /// no truncation yet.
 ///
@@ -93,11 +141,11 @@ private val expand_int:
 
 #set-options "--z3rlimit 10 --admit_smt_queries true"
 let rec expand_int #ha prk info len count curr previous =
-  if curr <^ len && FStar.UInt8.(count <^ 255uy) then (
+  if curr < len && FStar.UInt8.(count <^ 255uy) then (
     assert(FStar.UInt8.(count <^ 255uy));
     assert(UInt8.v count < 255);
     let count = FStar.UInt8.(count +^ 1uy) in
-    let curr = curr +^ tagLen ha in
+    let curr = curr + tagLen ha in
     lemma_repr_bytes_values (UInt8.v count);
     assume (UInt.fits (length previous + length info + 1) 32);
     let block = HMAC.hmac ha prk (previous @| info @| bytes_of_int8 count) in
@@ -126,6 +174,8 @@ let expand #ha prk info len =
   let rawbytes = expand_int prk info len 0uy 0ul empty_bytes in
   fst (split rawbytes len) 
 #reset-options
+*)
+
 
 (*-------------------------------------------------------------------*)
 (*
@@ -149,37 +199,46 @@ let tls13_prefix : lbytes 6 =
   let s = bytes_of_string "tls13 " in 
   assume(length s = 6); s
 
+let quic_prefix : lbytes 5 =
+  let s = bytes_of_string "quic " in
+  assume(length s = 5); s
+
+inline_for_extraction
 val format:
   ha: Hashing.alg -> 
   label: string{length (bytes_of_string label) < 256 - 6} -> 
   hv: bytes{length hv < 256} -> 
   len: UInt32.t {v len <= op_Multiply 255 (tagLength ha)} ->
+  is_quic: bool -> 
   Tot bytes
 
-let format ha label hv len = 
-  let label_bytes = tls13_prefix @| bytes_of_string label in
+inline_for_extraction
+let format ha label hv len is_quic = 
+  let prefix = if is_quic then quic_prefix else tls13_prefix in
+  let label_bytes = prefix @| bytes_of_string label in
   lemma_repr_bytes_values (v len);
   lemma_repr_bytes_values (length label_bytes);
   lemma_repr_bytes_values (length hv);
   bytes_of_int 2 (v len) @|
-  vlbytes 1 label_bytes @|
-  vlbytes 1 hv 
+  Parse.vlbytes 1 label_bytes @|
+  Parse.vlbytes 1 hv 
 
 /// since derivations depend on the concrete info,
 /// we will need to prove format injective. 
 
 val expand_label: 
-  #ha: Hashing.alg
-  -> prk: hkey ha
-  -> label: string{length (bytes_of_string label) < 256 - 6} // -9?
-  -> hv: bytes{length hv < 256}
-  -> len: UInt32.t {v len <= op_Multiply 255 (tagLength ha)}
-  -> ST (lbytes32 len)
+  #ha: HMAC.ha -> 
+  prk: hkey ha ->
+  label: string{length (bytes_of_string label) < 256 - 6} -> // -9?
+  hv: bytes{length hv < 256} ->
+  len: UInt32.t {v len <= op_Multiply 255 (tagLength ha)} ->
+  is_quic: bool ->
+  ST (lbytes32 len)
   (requires (fun h0 -> True))
   (ensures (fun h0 t h1 -> modifies_none h0 h1))
 
-let expand_label #ha prk label hv len =
-  expand prk (format ha label hv len) len
+let expand_label #ha prk label hv len is_quic =
+  expand prk (format ha label hv len is_quic) len 
 
 (*-------------------------------------------------------------------*)
 (*
@@ -190,7 +249,7 @@ let expand_label #ha prk label hv len =
 /// renamed to expand_secret for uniformity
 
 val expand_secret:
-  #ha:Hashing.alg ->
+  #ha: EverCrypt.HMAC.ha ->
   secret: hkey ha ->
   label: string{length (bytes_of_string label) < 256-6} ->
   hs_hash: bytes{length hs_hash < 256} ->
@@ -199,7 +258,7 @@ val expand_secret:
   (ensures fun h0 _ h1 -> modifies_none h0 h1)
 
 let expand_secret #ha prk label hv =
-  expand_label prk label hv (Hashing.Spec.tagLen ha)
+  expand_label prk label hv (Hashing.Spec.tagLen ha) false
   
 (*-------------------------------------------------------------------*)
 (*
@@ -209,22 +268,27 @@ let expand_secret #ha prk label hv =
              *)
 
 val derive_secret:
-  ha:hash_alg ->
+  ha: EverCrypt.HMAC.ha ->
   secret: hkey ha ->
   label: string{length (bytes_of_string label) < 256-6} ->
   hs_hash: bytes{length hs_hash < 256} ->
+  is_quic: bool -> 
   ST (lbytes32 (Hashing.Spec.tagLen ha))
   (requires fun h -> True)
   (ensures fun h0 _ h1 -> modifies_none h0 h1)
 
-let derive_secret ha secret label hashed_log =
-  let lbl = tls13_prefix @| bytes_of_string label in
-  cut(length lbl < 256);
-  lemma_repr_bytes_values (Hashing.Spec.tagLength ha);
+#set-options "--z3rlimit 200"
+let derive_secret ha secret label hashed_log is_quic =
+  let prefix = if is_quic then quic_prefix else tls13_prefix in
+  assert(length prefix <= 6);
+  let lbl = prefix @| bytes_of_string label in
+  assert(length lbl < 256);
+  let tlen = Hashing.Spec.tagLen ha in
+  lemma_repr_bytes_values (v tlen);
   lemma_repr_bytes_values (length lbl);
   lemma_repr_bytes_values (length hashed_log);
   let info =
-  bytes_of_int 2 (Hashing.Spec.tagLength ha) @|
-  vlbytes 1 lbl @|
-  vlbytes 1 hashed_log in
-  expand #ha secret info (Hashing.Spec.tagLen ha)
+    bytes_of_int 2 (v tlen) @|
+    Parse.vlbytes 1 lbl @|
+    Parse.vlbytes 1 hashed_log in
+  expand #ha secret info tlen
