src/tls/HMAC.fst
@@ -1,31 +1,135 @@
 ﻿module HMAC
 
-open FStar.Bytes
-open FStar.HyperStack.ST
-
-open Mem
-open TLSConstants
 open Hashing.Spec // for the algorithm names, instead of CoreCrypt
+open Mem
 
-#reset-options "--initial_fuel 0 --max_fuel 0 --initial_ifuel 0 --max_ifuel 0"
+open FStar.HyperStack.ST
+open FStar.Bytes
+
+let ha = EverCrypt.HMAC.ha 
 
 type key = bytes
-type mac (a:macAlg) = lbytes32 (macSize a)
+// type mac (a:macAlg) = lbytes32 (macSize a)
 //18-02-25 should instead be derived from Hashing
 
 type text (a:alg) = macable a
 
 (* Parametric keyed HMAC; could be coded up from two HASH calls. *)
 
-val hmac: a:alg -> k:hkey a -> m: macable a -> 
-  ST (t:tag a {t == Hashing.Spec.hmac a k m})
+(*
+// bytes input but uses a buffer for the resulting tag
+private val hmac0:
+  a:ha -> 
+  k:hkey a -> 
+  m: macable a -> 
+  bt: LowStar.Buffer.buffer UInt8.t {LowStar.Buffer.length bt = tagLength a} -> 
+  Stack unit
+  (requires fun h0 -> LowStar.Buffer.live h0 bt)
+  (ensures fun h0 () h1 -> 
+    LowStar.Buffer.as_seq h1 bt == Bytes.reveal (Hashing.Spec.hmac a k m) /\
+    LowStar.Modifies.(modifies (loc_buffer bt) h0 h1))
+
+let hmac0 a k m bt = 
+  let h00 = HyperStack.ST.get() in 
+  push_frame(); 
+  let h0 =  HyperStack.ST.get() in 
+  let lt = EverCrypt.Hash.tagLen a in
+  let bk = LowStar.Buffer.alloca 0uy lt in 
+  store_bytes k bk;
+  assert_norm(EverCrypt.HMAC.keysized a (tagLength a));
+
+  let lm = Bytes.len m in 
+  if lm = 0ul then (
+    let bm = LowStar.Buffer.null in 
+    EverCrypt.HMAC.compute a bt bk lt bm lm
+  )
+  else (
+    push_frame();
+    let bm = LowStar.Buffer.alloca 0uy lm in 
+    store_bytes m bm;
+    EverCrypt.HMAC.compute a bt bk lt bm lm;
+    pop_frame()
+    );
+  pop_frame();
+  assume False
+
+val hmac: 
+  a:ha -> 
+  k:hkey a -> 
+  m: macable a -> 
+  Stack (t:tag a {t == Hashing.Spec.hmac a k m})
   (requires (fun h0 -> True))
   (ensures (fun h0 t h1 -> FStar.HyperStack.modifies Set.empty h0 h1))
+  // TODO add functional spec to crypto proof 
+  
+let hmac a k m = 
+  let h00 = HyperStack.ST.get() in 
+  push_frame(); 
+  let lt = EverCrypt.Hash.tagLen a in
+  let bt = LowStar.Buffer.alloca 0uy lt in
+  hmac0 a k m bt; 
+  let t = of_buffer lt bt in
+  pop_frame();
+  let h11 = HyperStack.ST.get() in 
+  assume(HyperStack.modifies Set.empty h00 h11);
+  // assume(t = Hashing.Spec.hmac a k m);
+  t
 
-let hmac a k m = Hashing.OpenSSL.hmac a k m
+val hmac_verify: 
+  a:ha -> 
+  k:hkey a -> 
+  m: macable a -> 
+  t:tag a -> 
+  Stack (b:bool {b = (t = Hashing.Spec.hmac a k m)})
+  (requires (fun h0 -> True))
+  (ensures (fun h0 t h1 -> FStar.HyperStack.modifies Set.empty h0 h1))
+*)
 
-// consider providing it only in UFCMA
-val hmacVerify: a:alg -> k:hkey a -> m:macable a -> t: tag a -> ST (b:bool {b <==> (t == Hashing.Spec.hmac a k m)})
+val hmac:
+  a:ha -> 
+  k:hkey a -> 
+  m: macable a -> 
+  Stack (tag a)
+  (requires fun h0 -> True)
+  (ensures fun h0 t h1 -> 
+    modifies Set.empty h0 h1 /\
+    t = Hashing.Spec.hmac a k m)
+
+let hmac a k m = 
+  let h00 = HyperStack.ST.get() in 
+  push_frame(); 
+  let lt = EverCrypt.Hash.tagLen a in
+  let bk = LowStar.Buffer.alloca 0uy lt in 
+  store_bytes k bk;
+  assert_norm(EverCrypt.HMAC.keysized a (tagLength a));
+
+  let bt = LowStar.Buffer.alloca 0uy lt in
+  let lm = Bytes.len m in 
+
+  if lm = 0ul then (
+    let bm = LowStar.Buffer.null in 
+    EverCrypt.HMAC.compute a bt bk lt bm lm
+  )
+  else (
+    push_frame();
+    let bm = LowStar.Buffer.alloca 0uy lm in 
+    store_bytes m bm;
+    EverCrypt.HMAC.compute a bt bk lt bm lm;
+    pop_frame()
+    );
+  assume False;//18-09-01 not sure what's broken
+    
+  let t = of_buffer lt bt in
+  pop_frame();
+  let h11 = HyperStack.ST.get() in 
+  //18-09-01 todo, as in Hashing.compute
+  //assume(HyperStack.modifies Set.empty h00 h11);
+  t
+
+
+//18-09-02 TODO lower code to avoid bytes-allocating the tag. 
+
+val hmacVerify: a:ha -> k:hkey a -> m:macable a -> t: tag a -> ST (b:bool {b <==> (t == Hashing.Spec.hmac a k m)})
   (requires (fun h0 -> True))
   (ensures (fun h0 t h1 -> FStar.HyperStack.modifies Set.empty h0 h1))
 
@@ -34,8 +138,9 @@ let hmacVerify a k p t =
   result = t
 
 
-(* Historical constructions from SSL, still used in TLS 1.0, not that different from HMAC *)
-
+/// Historical constructions from SSL, still used in TLS 1.0, actually
+/// just HMAC. Disable in this version of the code.
+(*
 (* SSL/TLS constants *)
 
 private let ssl_pad1_md5  = create 48ul 0x36z
@@ -44,7 +149,7 @@ private let ssl_pad1_sha1 = create 40ul 0x36z
 private let ssl_pad2_sha1 = create 40ul 0x5cz
 
 (* SSL3 keyed hash *)
-type sslHashAlg = h:hashAlg { h = Hash MD5 \/ h = Hash SHA1 }
+type sslHashAlg = h:tls_alg { h = Hash MD5 \/ h = Hash SHA1 }
 val sslKeyedHashPads: sslHashAlg -> Tot(bytes * bytes)
 let sslKeyedHashPads = function
     | Hash MD5 -> (ssl_pad1_md5, ssl_pad2_md5)
@@ -60,6 +165,9 @@ let sslKeyedHash a k p =
       match a with 
       | MD5 -> ssl_pad1_md5, ssl_pad2_md5
       | SHA1 -> ssl_pad1_sha1, ssl_pad2_sha1 in
+
+    //18-08-31 TODO 4x hashable bounds
+    assume(False);
     let h = Hashing.compute a (k @| inner @| p) in
     Hashing.compute a (k @| outer @| h)
 
@@ -71,22 +179,29 @@ private val sslKeyedHashVerify:
 let sslKeyedHashVerify a k p t =
     let res = sslKeyedHash a k p in
     res=t
+*)
 
 
-(* Agile MAC function *)
+/// Agile bytes-friendly MAC function
 
-val tls_mac: a: macAlg -> k:lbytes32 (macKeySize a) -> msg:bytes -> ST (mac a)
-  (requires fun h0 -> match a with HMac a | SSLKHash a -> length msg + blockLength a <= maxLength a)
+type macable = b:bytes {length b + 128 < pow2 32} // [==> pre of hmac for all algorithms]
+
+val tls_mac: a: 
+  tls_macAlg -> 
+  k: tag a  -> 
+  msg:macable -> 
+  ST (tag a)
+  (requires fun h0 -> True)
   (ensures fun h0 t h1 -> FStar.HyperStack.modifies Set.empty h0 h1)
-let tls_mac a k msg  =
-    match a with
-    | HMac     a -> hmac a k msg
-    | SSLKHash a -> sslKeyedHash a k msg
+let tls_mac a k msg  = hmac a k msg
 
-val tls_macVerify: a:macAlg -> k:lbytes32 (macKeySize a) -> msg:bytes -> mac a -> ST bool
-  (requires fun h0 -> match a with HMac a | SSLKHash a -> length msg + blockLength a <= maxLength a)
+val tls_macVerify: 
+  a:tls_macAlg -> 
+  k: tag a  -> 
+  msg:macable -> 
+  tag a -> 
+  ST bool
+  (requires fun h0 -> True)
   (ensures (fun h0 t h1 -> FStar.HyperStack.modifies Set.empty h0 h1))
-let tls_macVerify a k d t =
-    match a with
-    | HMac alg -> hmacVerify alg k d t
-    | SSLKHash alg -> sslKeyedHashVerify alg k d t
+let tls_macVerify a k d t = hmacVerify a k d t
+
