src/tls/Hashing.Spec.fst
@@ -1,54 +1,44 @@
-﻿(** hash algorithms and providers *)
+﻿(** hash algorithms and providers
+
+ * provides bytes-friendly API before idealization
+ * no dependency on TLS: could go to EverCrypt or SecureAPI.
+
+*)
 module Hashing.Spec
 
-open FStar.UInt32
-open FStar.Bytes
+include EverCrypt.Hash 
 
-type alg = // CoreCrypto.hash_alg
-  | MD5
-  | SHA1
-  | SHA224
-  | SHA256
-  | SHA384
-  | SHA512
-//  | SHAKE128 of (n:nat{n >= 8})
-//  | SHAKE256 of (n:nat{n >= 16})
-// see e.g. https://en.wikipedia.org/wiki/SHA-1 for a global comparison and lengths
+open FStar.Integers
+open FStar.Bytes 
+type tag (a:alg) = Bytes.lbytes32 (tagLen a)
+type anyTag = lbytes (Integers.v maxTagLen)
 
-type alg13  = a:alg {a=SHA256 \/ a=SHA384 \/ a=SHA512}
+let macable a = b:bytes {length b + blockLength a < pow2 32}
+// 32-bit implementation restriction 
 
-let string_of_alg = function
-  | MD5    -> "MD5"
-  | SHA1   -> "SHA1"
-  | SHA224 -> "SHA224"
-  | SHA256 -> "SHA256"
-  | SHA384 -> "SHA384"
-  | SHA512 -> "SHA512"
+// HMAC specification
+// in contrast with RFC 2104 (which take any key length),
+// in TLS, the HMAC key has the same length as the hash [TLS1.3, 4.4.3]
 
-// length of the input blocks, in bytes (used for specifying the outer hash loop)
-let blockLen = function
-  | MD5 | SHA1 | SHA224 | SHA256 ->  64ul
-  | SHA384 | SHA512              -> 128ul
-//| SHAKE128 _ -> 168 | SHAKE256 _ -> 136
-let blockLength a = v (blockLen a)
+type hkey (a:alg) = tag a
 
-// length of the resulting tag, in bytes
-let maxTagLen = 64ul
-let tagLen (a:alg) : Tot (n:UInt32.t {n <=^ maxTagLen}) =
-  match a with
-  | MD5    -> 16ul
-  | SHA1   -> 20ul
-  | SHA224 -> 28ul // truncated SHA256
-  | SHA256 -> 32ul
-  | SHA384 -> 48ul // truncated SHA512
-  | SHA512 -> 64ul
-let tagLength a = v (tagLen a)
-//  | SHAKE128 d -> d
-//  | SHAKE256 d -> d
-type tag (a:alg) = lbytes32 (tagLen a)
-type anyTag = lbytes32 maxTagLen
-let lemma_maxLen (a:alg): Lemma (tagLen a <=^ maxTagLen) = ()
+val hmac: 
+  a:alg -> 
+  k:hkey a -> 
+  text:macable a -> 
+  GTot (t:tag a{
+    let text = Bytes.reveal text in 
+    Seq.length text + blockLength a <= maxLength a /\
+    Bytes.reveal t = EverCrypt.HMAC.hmac a (Bytes.reveal k) text})
 
+let hmac a k text = 
+  let k = Bytes.reveal k in 
+  let text = Bytes.reveal text in 
+  assert_norm (Seq.length text + blockLength a <= maxLength a);
+  let t: EverCrypt.Hash.tag a = EverCrypt.HMAC.hmac a k text in
+  Bytes.hide t
+
+//18-08-31 review
 // The hash of the empty string, used in KS
 #set-options "--admit_smt_queries true" //17-05-08 TODO size of bytes constants.
 let emptyHash : a:alg -> Tot (tag a) =
@@ -65,106 +55,24 @@ let emptyHash : a:alg -> Tot (tag a) =
 let zeroHash (a:alg): Tot (tag a) = Bytes.create (tagLen a) 0uy
 
 
-// internal hash state for incremental computation
-// with initial value and core algorithm, accumulating an extra block into the current state
+// TLS-specific hash and MAC algorithms (review) 
+type tls_alg = 
+  | NULL
+  | MD5SHA1
+  | Hash of alg
 
-// cwinter: keeping implementation so as not to break extraction.
-// assume type acc (a:alg)
-// assume val acc0: a:alg -> Tot (acc a)
-// assume val compress: #a:alg -> acc a -> lbytes32 (blockLen a) -> Tot (acc a)
-// assume val truncate: #a:alg -> acc a -> Tot (tag a) // just keeping the first tagLen bytes
+val tls_tagLen: h:tls_alg{h<>NULL} -> Tot UInt32.t
+let tls_tagLen = function
+  | Hash a  -> tagLen a
+  | MD5SHA1 -> tagLen MD5 + tagLen SHA1
 
-//18-02-26 TODO reconcile with fake abstract implementation in quic2c, which was:
+type tls_macAlg = EverCrypt.HMAC.ha
 
-//NS, JR: A very dubious change here, replacing an assumed type and functions on it
-//        Otherwise, this doesn't compile at all
-
-abstract
-let acc (a:alg) = bytes
-
-abstract
-let acc0 (a:alg) : acc a = empty_bytes
-
-abstract
-let compress (#a:alg) (_:acc a) (l:lbytes32 (blockLen a)) = l <: acc a //??
-
-module U32 = FStar.UInt32 
-
-abstract
-let truncate (#a:alg) (ac:acc a): Tot (lbytes32 (tagLen a)) =
-  let l = tagLen a in
-  assume (U32.(Bytes.len ac <=^ tagLen a));
-  assume (U32.(l <=^ Bytes.len ac));
-  let r = Bytes.slice ac 0ul l in
-  assume (U32.(len r =^ l));
-  r //?? just keeping the first tagLen bytes
-
-(*
-let acc0 = function
-  | MD5 ->  [0x67452301; 0xefcdab89; 0x98badcfe; 0x10325476] // A, B, C, D
-  | SHA1 -> [0x67452301; 0xefcdab89; 0x98badcfe; 0x10325476; 0xc3d2e1f0] // h0--h4
-  | SHA224 -> [0xc1059ed8; 0x367cd507; 0x3070dd17; 0xf70e5939; 0xffc00b31; 0x68581511; 0x64f98fa7; 0xbefa4fa4] // second 32 bits of the fractional parts of the square roots of the 9th through 16th primes 23..53
-  | SHA256 -> [0x6a09e667; 0xbb67ae85; 0x3c6ef372; 0xa54ff53a; 0x510e527f; 0x9b05688c; 0x1f83d9ab; 0x5be0cd19] // first 32 bits of the fractional parts of the square roots of the first 8 primes 2..19
-  | SHA384 -> [0xcbbb9d5dc1059ed8; 0x629a292a367cd507; 0x9159015a3070dd17; 0x152fecd8f70e5939; 0x67332667ffc00b31; 0x8eb44a8768581511; 0xdb0c2e0d64f98fa7; 0x47b5481dbefa4fa4]
-  | SHA512 -> [0x6a09e667f3bcc908; 0xbb67ae8584caa73b; 0x3c6ef372fe94f82b; 0xa54ff53a5f1d36f1; 0x510e527fade682d1; 0x9b05688c2b3e6c1f; 0x1f83d9abfb41bd6b; 0x5be0cd19137e2179]
-*)
-
-val hash2: #a:alg -> acc a -> b:bytes {length b % blockLength a = 0} -> Tot (acc a) (decreases (length b))
-let rec hash2 #a v b =
-  if len b = 0ul then v
-  else
-    let bl = blockLen a in
-    assume (U32.(0ul <=^ bl && bl <^ len b));
-    let c,b = split b bl in
-    hash2 (compress v c) b
-
-(** maximal input lengths for hashing and hmac, overly limited by our UInt32 of bytes lengths *)
-let maxLength a: nat = pow2 32 - blockLength a - 9
-let hashable a = b: bytes {length b <= maxLength a}
-let macable a = b: bytes {length b + blockLength a <= maxLength a}
-
-// for convenience, we treat inputs as sequences of bytes, not bits.
-// but note what's encoded in the suffix is the length in bits.
-private 
-let suffixLength (a:alg) (len:UInt32.t {v len <= maxLength a}): n:nat {(n + v len) % blockLength a = 0 /\ n <= blockLength a + 9} =
-  let blocklen = v (blockLen a) in 
-  let lenlen = match a with | SHA384 | SHA512 -> 8 | _ -> 4 in
-  let required = v len + 1 + lenlen in // minimal length after padding and encoding the length
-  let zeros = // minimal extra padding for block alignment
-    if required % blocklen = 0 
-    then 0
-    else blocklen - (required % blocklen) in
-    //was, harder to prove: required + blockLen a - ((required - 1) % blockLen a + 1) in
-  1 + zeros + lenlen
-
-// injective encoding for variable-length inputs
-// we add either 8 or 16 bytes of length and 1+ bytes of padding
-private 
-val suffix: a:alg -> len:UInt32.t {v len <= maxLength a} -> Tot (lbytes (suffixLength a len))
-// 2018.04.23 SZ: TODO: this is a placeholder, define properly
-let suffix a len =
- Bytes.create (FStar.UInt32.uint_to_t (suffixLength a len)) 0uy
-
-// computed in one step (specification)
-val hash: a:alg -> b:hashable a -> Tot (lbytes32 (tagLen a))
-let hash a b =
-  let q = suffix a (len b) in
-  assume (FStar.UInt.fits (length b + length q) 32);
-  let padded = b @| q in
-  let v = hash2 (acc0 a) padded in
-  let r = truncate v in
-  assert (U32.(len r <=^ tagLen a));
-  r
-
-// HMAC specification
-// in contrast with RFC 2104 (which take any key length),
-// in TLS, the HMAC key has the same length as the hash [TLS1.3, 4.4.3]
-type hkey (a:alg) = tag a
-
-val hmac: a:alg -> k:hkey a -> text:macable a -> Tot (tag a)
-let hmac a key message =
+(* for reference, a bytes spec of HMAC:
+let hmac a key message = EverCrypt.Hash. 
   let xkey = key @| create U32.(blockLen a -^ tagLen a) 0x0z  in
   let outer_key_pad = xor (blockLen a) xkey (create (blockLen a) 0x5cz) in
   let inner_key_pad = xor (blockLen a) xkey (create (blockLen a) 0x36z) in
   assume (FStar.UInt.fits (length inner_key_pad + length message) 32);
   hash a (outer_key_pad @| hash a (inner_key_pad @| message))
+*)
