src/tls/Range.fst
@@ -35,7 +35,7 @@ let ivSize i =
   let authEnc = aeAlg_of_id i in
   match authEnc with
   | MACOnly _ | MtE (Stream _) _ -> 0
-  | MtE (Block alg) _ -> CoreCrypto.blockSize alg
+  | MtE (Block alg) _ -> UInt32.v (EverCrypt.block_cipher_blockLen alg)
 
 (* Mandatory fixed padding for a cipher *)
 val fixedPadSize: id -> Tot nat
@@ -58,7 +58,7 @@ let maxPadSize i =
     | MtE (Block alg) _ ->
         lemma_MtE i; lemma_ID12 i;
         match pv_of_id i with
-          | SSL_3p0 -> CoreCrypto.blockSize alg
+          | SSL_3p0 -> UInt32.v (EverCrypt.block_cipher_blockLen alg)
           | TLS_1p0 | TLS_1p1 | TLS_1p2 -> 256
 
 (* Minimal padding length for a given plaintext length (in bytes) *)
@@ -70,7 +70,7 @@ let minimalPadding i len =
     match authEnc with
     | MACOnly _ | AEAD _ _ | MtE (Stream _) _ -> fixedPadSize i
     | MtE (Block alg) _ ->
-      let bs = CoreCrypto.blockSize alg in
+      let bs = UInt32.v (EverCrypt.block_cipher_blockLen alg) in
       let lp = len % bs in
       bs - lp
 
@@ -96,14 +96,14 @@ let valid_clen (i:id) (clen:nat) =
   else if ID13? i then
     begin
     lemma_ID13 i;
-    let tlen = CoreCrypto.aeadTagSize (aeAlg i) in
+    let tlen = UInt32.v (EverCrypt.aead_tagLen (aeAlg i)) in
     clen - tlen >= 0 &&
     clen - tlen <= max_TLSCiphertext_fragment_length_13
     end
   else // ID12? i
     begin
     if AEAD? (aeAlg_of_id i) then
-      let tlen = CoreCrypto.aeadTagSize (aeAlg i) in
+      let tlen = UInt32.v (EverCrypt.aead_tagLen (aeAlg i)) in
       clen - AE.explicit_iv_length i - tlen >= 0 &&
       clen - AE.explicit_iv_length i - tlen <= max_TLSPlaintext_fragment_length
     else if MtE? (aeAlg_of_id i) then
@@ -128,7 +128,7 @@ val cipherRangeClass: i:id2 -> clen:nat -> Pure range
     let (min, max) : range =
       match aeAlg_of_id i with
       | AEAD a _ ->
-        let x = clen - AE.explicit_iv_length i - CoreCrypto.aeadTagSize a in (x,x)
+        let x = clen - AE.explicit_iv_length i - UInt32.v (EverCrypt.aead_tagLen a) in (x,x)
       | MtE enc _ ->
         let m0 = clen - ivSize i - UInt32.v (macSize (macAlg_of_id i)) - maxPadSize i in
         let m1 = clen - ivSize i - UInt32.v (macSize (macAlg_of_id i)) - fixedPadSize i in
@@ -152,7 +152,7 @@ let cipherRangeClass i clen =
     min0 min, minP max
   | AEAD aeadAlg _ ->
     let ivL = AE.explicit_iv_length i in
-    let tagL = CoreCrypto.aeadTagSize aeadAlg in
+    let tagL = UInt32.v (EverCrypt.aead_tagLen aeadAlg) in
     let minmax = clen - ivL - tagL in
     minmax, minmax
 
@@ -209,7 +209,7 @@ let targetLength i (l,h) =
     cut(AEAD? (aeAlg_of_id i));
     let ivL = AE.explicit_iv_length i in
     cut(ivL >= 0);
-    let tagL = CoreCrypto.aeadTagSize aeadAlg in
+    let tagL = UInt32.v (EverCrypt.aead_tagLen aeadAlg) in
     cut(tagL >= 0);
     let fp = fixedPadSize i in
     cut(fp = 0);
